Set up improvements to type system definition
Making some of the conditions include completeness criteria, so they
will be more likely provable from what the contract type checker produces

Proofs are broken currently, to be repaired next

semantics/prop/vyperTypeInvariantsScript.sml
@@ -62,16 +62,67 @@ Definition fn_sigs_complete_def:
                 ret_ty := ret |>
 End
 
+Definition toplevel_vtypes_complete_def:
+  toplevel_vtypes_complete toplevel_vtypes cx <=>
+    (!src ts vis mut id ty init.
+       get_module_code cx src = SOME ts /\
+       MEM (VariableDecl vis mut id ty init) ts ==>
+       FLOOKUP toplevel_vtypes (src,string_to_num id) = SOME (Type ty)) /\
+    (!src ts vis is_transient id kt vt init.
+       get_module_code cx src = SOME ts /\
+       MEM (HashMapDecl vis is_transient id kt vt init) ts ==>
+       FLOOKUP toplevel_vtypes (src,string_to_num id) = SOME (HashMapT kt vt))
+End
+
+Definition is_bare_global_decl_def:
+  is_bare_global_decl n [] = F /\
+  is_bare_global_decl n (VariableDecl _ Immutable vid _ _ :: ts) =
+    (if string_to_num vid = n then T else is_bare_global_decl n ts) /\
+  is_bare_global_decl n (VariableDecl _ (Constant e) vid _ _ :: ts) =
+    (if string_to_num vid = n then T else is_bare_global_decl n ts) /\
+  is_bare_global_decl n (_ :: ts) = is_bare_global_decl n ts
+End
+
+Theorem is_immutable_decl_imp_is_bare_global_decl:
+  is_immutable_decl id ts ==> is_bare_global_decl id ts
+Proof
+  Induct_on `ts` >>
+  rw[is_immutable_decl_def, is_bare_global_decl_def] >>
+  Cases_on `h` >>
+  gvs[is_immutable_decl_def, is_bare_global_decl_def] >>
+  TRY (Cases_on `v0` >> gvs[is_immutable_decl_def, is_bare_global_decl_def])
+QED
+
+Definition bare_globals_complete_def:
+  bare_globals_complete bare_globals cx <=>
+    !src ts vis mut id ty init.
+      get_module_code cx src = SOME ts /\
+      MEM (VariableDecl vis mut id ty init) ts /\
+      (mut = Immutable \/ ?e. mut = Constant e) ==>
+      FLOOKUP bare_globals (src,string_to_num id) = SOME ty
+End
+
+Definition flag_members_complete_def:
+  flag_members_complete flag_members cx <=>
+    !src ts fid members.
+      get_module_code cx src = SOME ts /\
+      lookup_flag fid ts = SOME members ==>
+      FLOOKUP flag_members (src,fid) = SOME members
+End
+
 Definition env_context_consistent_def:
   env_context_consistent env cx <=>
     env.type_defs = get_tenv cx /\
     env.current_src = current_module cx /\
     fn_sigs_consistent env.fn_sigs cx /\
     fn_sigs_complete env.fn_sigs cx /\
+    toplevel_vtypes_complete env.toplevel_vtypes cx /\
+    bare_globals_complete env.bare_globals cx /\
+    flag_members_complete env.flag_members cx /\
     (!src id ty. FLOOKUP env.bare_globals (src,id) = SOME ty ==>
        ?ts. get_module_code cx src = SOME ts /\
             FLOOKUP env.toplevel_vtypes (src,id) = SOME (Type ty) /\
-            is_immutable_decl id ts /\
+            is_bare_global_decl id ts /\
             find_var_decl_by_num id ts = NONE /\
             ty <> NoneT) /\
     (!src id vt. FLOOKUP env.toplevel_vtypes (src,id) = SOME vt ==>
@@ -97,12 +148,21 @@ Definition env_context_consistent_def:
             FLOOKUP (get_tenv cx) (string_to_num fid) = SOME (FlagArgs (LENGTH ls)))
 End
 
+Theorem env_context_consistent_static_completeness:
+  env_context_consistent env cx ==>
+    toplevel_vtypes_complete env.toplevel_vtypes cx /\
+    bare_globals_complete env.bare_globals cx /\
+    flag_members_complete env.flag_members cx
+Proof
+  rw[env_context_consistent_def]
+QED
+
 Theorem env_context_consistent_bare_global_old:
   env_context_consistent env cx /\
   FLOOKUP env.bare_globals (src,id) = SOME ty /\
   get_module_code cx src = SOME ts ==>
     FLOOKUP env.toplevel_vtypes (src,id) = SOME (Type ty) /\
-    is_immutable_decl id ts /\ ty <> NoneT
+    is_bare_global_decl id ts /\ ty <> NoneT
 Proof
   rw[env_context_consistent_def] >>
   first_x_assum drule >> rw[] >> gvs[]
@@ -113,7 +173,7 @@ Theorem env_context_consistent_bare_global_find_NONE:
   FLOOKUP env.bare_globals (src,id) = SOME ty ==>
     ?ts. get_module_code cx src = SOME ts /\
          FLOOKUP env.toplevel_vtypes (src,id) = SOME (Type ty) /\
-         is_immutable_decl id ts /\
+         is_bare_global_decl id ts /\
          find_var_decl_by_num id ts = NONE /\
          ty <> NoneT
 Proof
@@ -170,7 +230,7 @@ Theorem env_consistent_bare_global_find_NONE:
   FLOOKUP env.bare_globals (src,id) = SOME ty ==>
     ?ts. get_module_code cx src = SOME ts /\
          FLOOKUP env.toplevel_vtypes (src,id) = SOME (Type ty) /\
-         is_immutable_decl id ts /\
+         is_bare_global_decl id ts /\
          find_var_decl_by_num id ts = NONE /\
          ty <> NoneT
 Proof
@@ -184,10 +244,13 @@ Definition functions_well_typed_def:
     !fn_sigs bare_globals toplevel_vtypes flag_members.
       fn_sigs_consistent fn_sigs cx /\
       fn_sigs_complete fn_sigs cx /\
+      toplevel_vtypes_complete toplevel_vtypes cx /\
+      bare_globals_complete bare_globals cx /\
+      flag_members_complete flag_members cx /\
       (!src id ty. FLOOKUP bare_globals (src,id) = SOME ty ==>
          ?ts. get_module_code cx src = SOME ts /\
               FLOOKUP toplevel_vtypes (src,id) = SOME (Type ty) /\
-              is_immutable_decl id ts /\
+              is_bare_global_decl id ts /\
               find_var_decl_by_num id ts = NONE /\
               ty <> NoneT) /\
       (!src id vt ts.
